Got unicity of sorting, restricted sum and get rid of let in

proof/CCPD.alaChen/Generation.v
@@ -7,6 +7,9 @@ Require Import Env.
 Require Import CCPD.Types.
 Require Import CCPD.Thinning.
 Require Import CCPD.Substitution.
+Require Import CCPD.Coercion.
+Require Import CCPD.GenerationNotKind.
+Require Import CCPD.GenerationCoerce.
 
 Implicit Types i k m n p : nat.
 Implicit Type s : sort.
@@ -14,526 +17,6 @@ Implicit Types A B M N T t u v : term.
 Implicit Types e f g : env.
 
 Set Implicit Arguments.
-
-Lemma lift_rec_eq_sort : forall t n k s, lift_rec n t k = Srt s -> t = Srt s.
-Proof.
-induction t ; simpl ; intros ; auto with coc core ; try discriminate.
-
-generalize H ; clear H ; elim (le_gt_dec k n) ; intros ; discriminate.
-Qed.
-
-Lemma lift_eq_sort : forall t n s, lift n t = Srt s -> t = Srt s.
-Proof.
-unfold lift ; intros ; apply lift_rec_eq_sort with n 0 ; auto.
-Qed.
-
-Lemma typ_not_kind : forall G t T, G |- t : T -> t <> Srt kind.
-Proof.
-red ; intros.
-rewrite H0 in H.
-pose (typ_sort _ _ _ H).
-induction a.
-unfold is_prop in H1.
-induction H1 ; discriminate.
-Qed.
-
-Lemma typ_not_kind2 : forall G T, ~ G |- Srt kind : T.
-Proof.
-  unfold not ; intros.
-  apply (typ_not_kind H).
-  auto.
-Qed.
-
-Hint Resolve lift_eq_sort typ_not_kind2 : coc.
-
-
-Fixpoint type_range (t : term) : term :=
-  match t with
-  | Prod U V => type_range V
-  | Sum U V => type_range V
-  | _ => t
-  end.
-
-Definition type_dom (t : term) : term :=
-  match t with
-  | Prod U V => type_range U
-  | Sum U V => type_range U
-  | _ => type_range t
-  end.
-
-Fixpoint type_no_kind (t : term) : Prop :=
-  match t with
-  | Prod U V => type_no_kind U /\ type_no_kind V
-  | Sum U V => type_no_kind U /\ type_no_kind V
-  | Srt kind => False
-  | _ => True
-  end.
-
-Lemma type_has_no_kind : forall G t T, G |- t : T -> type_no_kind t.
-Proof.
-  induction 1; simpl ; intros ; auto with coc ; try discriminate.
-Qed.
-
-Lemma type_no_kind_not_kind : forall t, type_no_kind t -> t <> Srt kind.
-Proof.
-  induction t ; unfold not ; intros ; try discriminate.
-  simpl in H.
-  inversion H0.
-  rewrite H2 in H.
-  auto.
-Qed.
-(*
-Lemma type_range_not_kind_ps : forall G t T, G |- t : T -> 
-  forall U V, t = Prod U V \/ t = Sum U V -> type_range U <> Srt kind /\
-  type_range V <> Srt kind.
-Proof.
-  induction 1; simpl ; intros ; auto with coc ; try (intuition ; discriminate).
-  destruct H1.
-
-  inversion H1.
-  rewrite <- H3.
-  rewrite <- H4.
-  split.
-  apply (type_range_not_kind H).
-  apply (type_range_not_kind H0).
-  discriminate.
-
-  inversion H1.
-  discriminate.
-  inversion H2.
-  rewrite <- H4.
-  rewrite <- H5.
-  split.
-  apply (type_range_not_kind H).
-  apply (type_range_not_kind H0).
-Qed.
-*)
-Lemma lift_type_range_eq_sort : forall n t k, type_no_kind (lift_rec n t k) -> 
-  type_no_kind t.
-Proof.
-  induction t ; simpl ; intros ; try discriminate ; auto.
-
-  intuition.
-  apply IHt1 with k ; auto.
-  apply IHt2 with (S k) ; auto.
-
-  intuition.
-  apply IHt1 with k ; auto.
-  apply IHt2 with (S k) ; auto.
-Qed.
-
-Lemma type_no_kind_lift : forall n t k, type_no_kind t ->
-  type_no_kind (lift_rec n t k).
-Proof.
-  induction t ; simpl ; intros ; try discriminate ; auto.
-
-  elim (le_gt_dec k n0) ; simpl ; intros ; auto.
-  intuition.
-  intuition.
-Qed.
-
-Lemma type_range_subst_not_kind : forall u v n, type_no_kind u ->
-  type_no_kind v -> type_no_kind (subst_rec u v n).
-Proof.
-  induction v ; simpl ; intros ; try discriminate ; auto.
-
-  elim (lt_eq_lt_dec n0 n) ; intros.
-  induction a ; simpl ; intros ; unfold not ; intros ; try discriminate ; auto.
-  unfold lift ; apply (type_no_kind_lift); auto.
-  auto.
-
-  intuition.
-  intuition.
-Qed.
- 
-Lemma type_no_kind_type : forall G t T, G |- t : T -> 
-  forall U V, (T = Prod U V \/ T = Sum U V) -> type_no_kind T.
-Proof.
-  induction 1 using typ_mutwf with
-  (P := fun G t T => fun H : G |- t : T =>
-  forall U V, (T = Prod U V \/ T = Sum U V) -> type_no_kind T)
-  (P0 := fun G U V s => fun H : G |- U >> V : s => True (*
-    (forall X Y, U = Prod X Y -> prod_sort Y <> Srt kind) /\
-    (forall X Y, U = Prod X Y -> prod_sort Y <> Srt kind)*))
-  (P1 := fun e => fun H : wf e => 
-    forall T n, item_lift T e n -> 
-    forall U V, (T = Prod U V \/ T = Sum U V) -> type_no_kind T)
- ; simpl ; intros ; auto with coc ; try discriminate ; 
- try (destruct H ; discriminate) ;  try (destruct H1 ; discriminate).
-
-  apply IHtyp with n U V ; auto.
-
-  destruct H2 ; try discriminate.
-  assert (e |- Prod T U : Srt s2).
-  apply type_prod with s1 ; auto with coc.
-  pose (type_has_no_kind H3) ; auto with coc.
-
-  destruct H1.
-  induction Ur ;  try (unfold subst, subst_rec ; simpl ; intros ; discriminate).
-  unfold subst in H1.
-  generalize H1 ; clear H1.
-  unfold subst_rec ; elim (lt_eq_lt_dec 0 n).
-  intro a ; case a ; clear a ; intros ; try discriminate.
-  rewrite <- e0 ; simpl.
-  unfold subst ; simpl.
-  rewrite lift0.
-  apply (type_has_no_kind H) ; auto with coc.
-
-  intros ; discriminate.
-  pose (IHtyp2 V (Prod Ur1 Ur2) (or_introl _ (refl_equal (Prod V (Prod Ur1 Ur2))))).
-  simpl in t.
-  destruct t.
-  destruct H3.
-  unfold subst in H1 ; simpl in H1.
-  clear IHUr1 IHUr2.
-
-  inversion H1.
-
-  pose (type_has_no_kind H).
-  split ; apply type_range_subst_not_kind ; auto.
-
-  induction Ur ;  try (unfold subst, subst_rec ; simpl ; intros ; discriminate).
-  unfold subst in H1.
-  generalize H1 ; clear H1.
-  unfold subst_rec ; elim (lt_eq_lt_dec 0 n).
-  intro a ; case a ; clear a ; intros ; try discriminate.
-  rewrite <- e0 ; simpl.
-  unfold subst ; simpl.
-  rewrite lift0.
-  apply (type_has_no_kind H) ; auto with coc.
-
-  intros ; discriminate.
-  pose (IHtyp2 V (Sum Ur1 Ur2) (or_introl _ (refl_equal (Prod V (Sum Ur1 Ur2))))).
-  simpl in t.
-  destruct t.
-  destruct H3.
-  unfold subst in H1 ; simpl in H1.
-  clear IHUr1 IHUr2.
-
-  inversion H1.
-
-  pose (type_has_no_kind H).
-  split ; apply type_range_subst_not_kind ; auto.
-
-  destruct H3.
-  discriminate.
-  inversion H3.
-  rewrite <- H6.
-  rewrite <- H5.
-  split ; [apply (type_has_no_kind H) | apply (type_has_no_kind H1)].
-  
-  pose (IHtyp U V (or_intror _ (refl_equal (Sum U V)))).
-  simpl in t0.
-  intuition.
-  
-  assert(type_no_kind (Pi1 t)) ; auto with coc.
-  simpl ; auto.
-  unfold subst ; apply type_range_subst_not_kind ; auto.
-  intuition.
-  pose (IHtyp U V (or_intror _ (refl_equal (Sum U V)))).
-  simpl in t0 ; intuition.
-  pose (IHtyp U V (or_intror _ (refl_equal (Sum U V)))).
-  simpl in t0 ; intuition.
-    
-  induction M ; intuition ; try discriminate.
-  generalize H4 ; unfold subst, subst_rec.
-  elim (lt_eq_lt_dec 0 n) ; intros a ; try discriminate.
-  case a ; clear a ; intros ; try discriminate.
-  rewrite lift0. rewrite lift0 in H3.
-  rewrite H3 ; rewrite H3 in H.
-  pose (type_has_no_kind H) ; auto with coc.
-  
-  intros ; discriminate.
-  pose (type_has_no_kind H2).
-  pose (type_has_no_kind H).
-  unfold subst ; apply type_range_subst_not_kind ; auto.
-  
-  unfold subst in H4 ; simpl in H4.
-  inversion H4.
-  pose (type_has_no_kind H2).
-  pose (type_has_no_kind H).
-  unfold subst ; apply type_range_subst_not_kind ; auto.
-
-  unfold subst in H4 ; simpl in H4.
-  inversion H4.
-  pose (type_has_no_kind H2).
-  pose (type_has_no_kind H).
-  unfold subst ; apply type_range_subst_not_kind ; auto.
-  
-  destruct H2 ;
-  rewrite H2 in H0 ;
-  rewrite H2 ; apply (type_has_no_kind H0).
-
-  destruct H.
-  elim (inv_nth_nl _ _ _ H1).
-  
-  assert (wf (T :: e)). 
-  apply wf_var with s ; auto with coc.
-  destruct (wf_sort_lift _ (T :: e) _ H2 H0).
-  apply (type_has_no_kind H3).
-Qed.
-
-Lemma type_no_kind_prod_type : forall G t U V, 
-  G |- t : Prod U V -> type_no_kind V.
-Proof.
-  intros.
-  pose (type_no_kind_type H (or_introl _ (refl_equal (Prod U V)))).
-  simpl in t0.
-  intuition.
-Qed.
-
-Lemma type_no_kind_prod_type2 : forall G t U V, 
-  G |- t : Prod U V -> type_no_kind (Prod U V).
-Proof.
-  intros.
-  pose (type_no_kind_type H (or_introl _ (refl_equal (Prod U V)))).
-  simpl in t0.
-  intuition.
-  simpl ; auto.
-Qed.
-
-Lemma type_no_kind_prod_type_sort : forall G t U V, 
-  G |- t : Prod U V -> 
-  forall s, type_range V = Srt s -> s <> kind.
-Admitted.
-
-Lemma type_no_kind_sum_type : forall G t U V, 
-  G |- t : Sum U V -> type_no_kind V.
-Proof.
-  intros.
-  pose (type_no_kind_type H (or_intror _ (refl_equal (Sum U V)))).
-  simpl in t0.
-  intuition.
-Qed.
-
-Definition is_low_sort (s : term) := s = Srt set \/ s = Srt prop.
-
-Lemma subst_to_sort : forall t t' s, subst t t' = Srt s -> t <> Srt s ->
-  t' = Srt s.
-Proof.
-  induction t' ; intros ; try discriminate.
-  unfold subst, subst_rec in H.
-  assumption.
-
-  unfold subst, subst_rec in H.
-  generalize H.
-  elim (lt_eq_lt_dec 0 n).
-  intros a.
-  induction a.
-  intros ; discriminate.
-  intros.
-  rewrite lift0 in H1.
-  contradiction.
-
-  intros ; discriminate.
-Qed.
-
-Lemma kind_is_prod : forall G t T, G |- t : T -> T = Srt kind ->
-  is_low_sort (type_range t).
-Proof.
-  induction 1 ; intros ; try discriminate ; simpl ; auto.
-  unfold is_low_sort ; intuition.
-  unfold is_low_sort ; intuition.
-  induction (wf_sort_lift _ _ _ H H0).
-  rewrite H1 in H2.
-  elim (typ_not_kind H2) ; auto.
-  
-  pose (subst_to_sort _ H1 (typ_not_kind H)).
-
-  pose (type_no_kind_type H0 (or_introl _ (refl_equal (Prod V Ur)))).
-  simpl in t.
-  destruct t.
-  rewrite e0 in H3.
-  simpl in H3.
-  contradiction.
-
-  pose (type_no_kind_type H (or_intror _ (refl_equal (Sum U V)))).
-  simpl in t0.
-  destruct t0.
-  rewrite H0 in H1.
-  simpl in H1.
-  contradiction.
-
-  pose (type_no_kind_type H (or_intror _ (refl_equal (Sum U V)))).
-  simpl in t0.
-  destruct t0.
-  assert(Pi1 t <> Srt kind) ; try (unfold not ; intros ; discriminate).
-  pose (subst_to_sort _ H0 H3).
-  rewrite e0 in H2.
-  simpl in H2.
-  contradiction.
-
-  pose (type_has_no_kind H).
-  pose (type_has_no_kind H2).
-  unfold subst in H3.
-  pose (type_range_subst_not_kind _ _ 0 t0 t1).
-  pose (type_no_kind_not_kind t2).
-  contradiction.
-
-  rewrite H3 in H0.
-  pose (typ_not_kind H0).
-  elim n ; auto.
-Qed.
-
-Lemma red_sort_eq : forall s t, red (Srt s) t -> t = Srt s.
-Proof.
-  simple induction 1; intros; auto with coc core arith sets.
-  rewrite H1 in H2.
-  inversion H2.
-Qed.
-
-Lemma sort_conv_eq : forall G T s, G |- T : Srt kind -> conv T (Srt s) -> T = Srt s.
-Proof.
-  intros.
-  destruct (church_rosser _ _ H0).
-  pose (red_sort_eq H2).
-  rewrite e in H1.
-
-  pose (kind_is_prod H (refl_equal (Srt kind))).
-  unfold is_low_sort in i.
-  induction T ; try (simpl in i ; destruct i ; inversion H1 ; try discriminate) ; auto with coc core.
-
-  rewrite (conv_sort _ _ H0).
-  auto.
-
-  rewrite (conv_sort _ _ H0).
-  auto.
-
-  pose (conv_sort_prod s T1 T2).
-  pose (sym_conv _ _ H0).
-  contradiction.
-
-  pose (conv_sort_prod s T1 T2).
-  pose (sym_conv _ _ H0).
-  contradiction.
-
-  pose (conv_sort_sum s T1 T2).
-  pose (sym_conv _ _ H0).
-  contradiction.
-
-  pose (conv_sort_sum s T1 T2).
-  pose (sym_conv _ _ H0).
-  contradiction.
-Qed.
-
-Lemma coerce_prop_sort_l_aux : forall G Ts A s', G |- Ts >> A : s' ->
-  Ts = Srt prop ->  s' = kind -> G |- A : Srt kind -> A = Srt prop.
-Proof.
-  induction 1 ; simpl ; intros ; try discriminate.
-  apply sort_conv_eq with e ; auto.
-  rewrite H2 in H1 ; auto with coc.
-
-  apply IHcoerce2 ; auto.
-  apply IHcoerce1 ; auto.
-  rewrite H2 in H0.
-  apply coerce_sort_l with C ; auto.
-Qed.
-
-Lemma coerce_set_sort_l_aux : forall G Ts A s', G |- Ts >> A : s' ->
-  Ts = Srt set ->  s' = kind -> G |- A : Srt kind -> A = Srt set.
-Proof.
-  induction 1 ; simpl ; intros ; try discriminate.
-  apply sort_conv_eq with e ; auto.
-  rewrite H2 in H1 ; auto with coc.
-
-  apply IHcoerce2 ; auto.
-  apply IHcoerce1 ; auto.
-  rewrite H2 in H0.
-  apply coerce_sort_l with C ; auto.
-Qed.
-
-
-Lemma coerce_prop_sort_r_aux : forall G Ts A s', G |- A >> Ts : s' ->
-  Ts = Srt prop ->  s' = kind -> G |- A : Srt kind -> A = Srt prop.
-Proof.
-  induction 1 ; simpl ; intros ; try discriminate.
-  apply sort_conv_eq with e ; auto.
-  rewrite H2 in H1 ; auto with coc.
-
-  apply IHcoerce1 ; auto.
-  apply IHcoerce2 ; auto.
-  rewrite H2 in H0.
-  apply coerce_sort_l with C ; auto.
-Qed.
-
-Lemma coerce_set_sort_r_aux : forall G Ts A s', G |- A >> Ts : s' ->
-  Ts = Srt set ->  s' = kind -> G |- A : Srt kind -> A = Srt set.
-Proof.
-  induction 1 ; simpl ; intros ; try discriminate.
-  apply sort_conv_eq with e ; auto.
-  rewrite H2 in H1 ; auto with coc.
-
-  apply IHcoerce1 ; auto.
-  apply IHcoerce2 ; auto.
-  rewrite H2 in H0.
-  apply coerce_sort_l with C ; auto.
-Qed.
-
-Lemma coerce_prop_sort_l : forall G A, G |- Srt prop >> A : kind -> A = Srt prop.
-Proof. 
-  intros.
-  eapply coerce_prop_sort_l_aux with G (Srt prop) kind ; auto.
-  apply coerce_sort_r with (Srt prop) ; auto.
-Qed.
-
-Lemma coerce_prop_sort_r : forall G A, G |- A >> Srt prop : kind -> A = Srt prop.
-Proof. 
-  intros.
-  eapply coerce_prop_sort_r_aux with G (Srt prop) kind ; auto.
-  apply coerce_sort_l with (Srt prop) ; auto.
-Qed.
-
-Lemma coerce_set_sort_l : forall G A, G |- Srt set >> A : kind -> A = Srt set.
-Proof. 
-  intros.
-  eapply coerce_set_sort_l_aux with G (Srt set) kind ; auto.
-  apply coerce_sort_r with (Srt set) ; auto.
-Qed.
-
-Lemma coerce_set_sort_r : forall G A, G |- A >> Srt set : kind -> A = Srt set.
-Proof. 
-  intros.
-  eapply coerce_set_sort_r_aux with G (Srt set) kind ; auto.
-  apply coerce_sort_l with (Srt set) ; auto.
-Qed.
-
-Lemma coerce_propset_l : forall G A s s', G |- Srt s >> A : s' -> A = Srt s.
-Proof.
-  intros.
-  assert(s' = kind).
-  pose (coerce_sort_l _ _ _ _ H).
-  pose (typ_sort _ _ _ t).
-  intuition.
-  inversion H1 ; auto.
-  rewrite H0 in H.
-  clear H0.
-  induction s.
-  pose (coerce_sort_l _ _ _  _ H).
-  pose (typ_not_kind t).
-  elim n ; auto.
-  
-  eapply coerce_prop_sort_l with G ; auto with coc.
-  eapply coerce_set_sort_l with G ; auto with coc.
-Qed.
-
-Lemma coerce_propset_r : forall G A s s', G |- A >> Srt s : s' -> A = Srt s.
-Proof.
-  intros.
-  assert(s' = kind).
-  pose (coerce_sort_r _ _ _ _ H).
-  pose (typ_sort _ _ _ t).
-  intuition.
-  inversion H1 ; auto.
-  rewrite H0 in H.
-  clear H0.
-  induction s.
-  pose (coerce_sort_r _ _ _  _ H).
-  pose (typ_not_kind t).
-  elim n ; auto.
-  
-  eapply coerce_prop_sort_r with G ; auto with coc.
-  eapply coerce_set_sort_r with G ; auto with coc.
-Qed.
 
 
 Lemma wf_is_sorted : forall e, wf e ->
@@ -754,34 +237,33 @@ Proof.
 Qed.
 
 Lemma generation_sum2_aux : forall e T Ts, e |- T : Ts ->
-  forall U V, T = Sum U V -> forall s, Ts = Srt s ->
-  (exists s', e |- U : Srt s') /\ (U :: e) |- V : Srt s.
+  forall U V, T = Sum U V -> forall s, Ts = Srt s -> 
+  exists s', e |- U : Srt s' /\ (U :: e) |- V : Srt s /\ sum_sort U V s' s.
 Proof.
   induction 1 ; simpl ; intros ; try discriminate.
 
-  inversion H1.
-  rewrite H4 in H.
-  rewrite H5 in H0.
-  rewrite H4 in H0.
-
-  split.
-  exists s1 ; auto.
   inversion H2.
-  rewrite <- H6.
-  assumption.
+  rewrite H3 in H0.
+  rewrite H6 in H0.
+  rewrite H5 in H0.
+
+  exists s1.
+  rewrite <- H5.
+  split ; auto.
+  inversion H3.
+  rewrite <- H5 in H0.
+  rewrite H7 in H1.
+  rewrite H6 in H1.
+  split ; auto.
 
   rewrite H4 in H2.
-  rewrite H4 in H0.
-  induction (typ_sort _ _  _ H0).
-  inversion H6.
-  rewrite H8 in H2.
   pose (coerce_propset_r H2).
 
-  apply (IHtyp1 U0 V0 H3 s0 e0).
+  apply (IHtyp1 U0 V0 H3 s0 e0) ; auto.
 Qed.
 
 Lemma generation_sum2 : forall e U V s, e |- Sum U V : Srt s ->
-  (exists s', e |- U : Srt s') /\ (U :: e) |- V : Srt s.
+  exists s', e |- U : Srt s' /\ (U :: e) |- V : Srt s /\ sum_sort U V s' s.
 Proof.
   intros.
   eapply generation_sum2_aux  ; auto ; auto.
@@ -885,6 +367,9 @@ Proof.
 
   elim conv_sort_sum with s A1 A2 ; auto with coc core.
   elim conv_sort_sum with s A1 A2 ; auto with coc core.
+
+  elim conv_sort_subset with s A1 A2 ; auto with coc core.
+  elim conv_sort_subset with s A1 A2 ; auto with coc core.
 Qed.
 
 Lemma conv_is_low_range_full : forall A B, conv A B ->
@@ -981,6 +466,10 @@ Proof.
   unfold is_low_sort ; rewrite H2 ; auto.
   unfold is_low_sort ; rewrite H0 ; auto.
 Qed.
+(*
+Lemma conv_sum_subset : forall A B C D, ~ conv (Sum A B) (Subset C D).
+Admitted.
+
 
 Lemma conv_is_low_dom_full : forall A B, conv A B ->
   is_low_sort (type_dom A) -> 
@@ -1012,12 +501,16 @@ Proof.
   unfold is_low_sort ; rewrite H0 ; auto.
 
   simpl in H0.
-  apply (IHA1 B1 (inv_conv_prod_l _ _ _ _ H)).
-  unfold is_low_sort ; rewrite H2 ; auto.
-  unfold is_low_sort ; rewrite H0 ; auto.
+  rewrite <- H2 ; rewrite <- H0.
+  apply (conv_is_low_range_full (inv_conv_prod_l _ _ _ _ H)).
+  rewrite H2 ; unfold is_low_sort ; auto.
+  rewrite H0 ; unfold is_low_sort ; auto.
 
   elim conv_prod_sum with A1 A2 B1 B2 ; auto with coc.
   elim conv_prod_sum with A1 A2 B1 B2 ; auto with coc.
+
+  elim conv_prod_subset with A1 A2 B1 B2 ; auto with coc.
+  elim conv_prod_subset with A1 A2 B1 B2 ; auto with coc.
 
   induction B ; simpl ; intros ; 
   try unfold is_low_sort in H1 ;   
@@ -1027,17 +520,22 @@ Proof.
   elim conv_sort_prod with s A1 A2 ; auto with coc core.
 
   simpl in H0.
-  apply (IHA2 B2 (inv_conv_prod_r _ _ _ _ H)).
-  unfold is_low_sort ; rewrite H2 ; auto.
-  unfold is_low_sort ; rewrite H0 ; auto.
+  rewrite H0 ; rewrite H2 ; auto.
+  
+  simpl in H0.
+  rewrite <- H2 ; rewrite <- H0.
+  apply (conv_is_low_range_full (inv_conv_prod_l _ _ _ _ H)).
+  rewrite H2 ; unfold is_low_sort ; auto.
+  rewrite H0 ; unfold is_low_sort ; auto.
 
   simpl in H0.
-  apply (IHA2 B2 (inv_conv_prod_r _ _ _ _ H)).
-  unfold is_low_sort ; rewrite H2 ; auto.
-  unfold is_low_sort ; rewrite H0 ; auto.
+  rewrite H2 ; rewrite H0 ; auto.
 
   elim conv_prod_sum with A1 A2 B1 B2 ; auto with coc.
   elim conv_prod_sum with A1 A2 B1 B2 ; auto with coc.
+
+  elim conv_prod_subset with A1 A2 B1 B2 ; auto with coc.
+  elim conv_prod_subset with A1 A2 B1 B2 ; auto with coc.
 
   induction B ; simpl ; intros ; 
   try unfold is_low_sort in H1 ;   
@@ -1046,18 +544,21 @@ Proof.
   elim conv_sort_sum with s A1 A2 ; auto with coc core.
   elim conv_sort_sum with s A1 A2 ; auto with coc core.
 
-  elim conv_prod_sum with B1 B2 A1 A2; auto with coc core.
-  elim conv_prod_sum with B1 B2 A1 A2; auto with coc core.
+  simpl in H0.
+  rewrite H0 ; rewrite H2 ; auto.
+  
+  elim conv_prod_sum with B1 B2 A1 A2 ; auto with coc core.
+  
+  simpl in H0.
+  rewrite H2 ; rewrite H0 ; auto.
 
   simpl in H0.
-  apply (IHA2 B2 (inv_conv_sum_r _ _ _ _ H)).
-  unfold is_low_sort ; rewrite H2 ; auto.
-  unfold is_low_sort ; rewrite H0 ; auto.
+  apply (conv_is_low_range_full (inv_conv_sum_l _ _ _ _ H)).
+  rewrite H2 ; unfold is_low_sort ; auto.
+  rewrite H0 ; unfold is_low_sort ; auto.
 
-  simpl in H0.
-  apply (IHA2 B2 (inv_conv_sum_r _ _ _ _ H)).
-  unfold is_low_sort ; rewrite H2 ; auto.
-  unfold is_low_sort ; rewrite H0 ; auto.
+  elim conv_sum_subset with A1 A2 B1 B2 ; auto with coc.
+  elim conv_sum_subset with A1 A2 B1 B2 ; auto with coc.
 
   induction B ; simpl ; intros ; 
   try unfold is_low_sort in H1 ;   
@@ -1066,20 +567,63 @@ Proof.
   elim conv_sort_sum with s A1 A2 ; auto with coc core.
   elim conv_sort_sum with s A1 A2 ; auto with coc core.
 
-  elim conv_prod_sum with B1 B2 A1 A2; auto with coc core.
-  elim conv_prod_sum with B1 B2 A1 A2; auto with coc core.
+  elim conv_prod_sum with B1 B2 A1 A2 ; auto with coc core.
+  elim conv_prod_sum with B1 B2 A1 A2 ; auto with coc core.
 
   simpl in H0.
-  apply (IHA2 B2 (inv_conv_sum_r _ _ _ _ H)).
-  unfold is_low_sort ; rewrite H2 ; auto.
-  unfold is_low_sort ; rewrite H0 ; auto.
+  apply (conv_is_low_range_full (inv_conv_sum_l _ _ _ _ H)).
+  rewrite H2 ; unfold is_low_sort ; auto.
+  rewrite H0 ; unfold is_low_sort ; auto.
 
   simpl in H0.
-  apply (IHA2 B2 (inv_conv_sum_r _ _ _ _ H)).
-  unfold is_low_sort ; rewrite H2 ; auto.
-  unfold is_low_sort ; rewrite H0 ; auto.
+  rewrite H2 ; rewrite H0 ; auto.
+
+
+  elim conv_sum_subset with A1 A2 B1 B2 ; auto with coc.
+  elim conv_sum_subset with A1 A2 B1 B2 ; auto with coc.
+  induction B ; simpl ; intros ; 
+  try unfold is_low_sort in H1 ;   
+  intuition ; try discriminate ; auto with coc core datatypes.
+
+  elim conv_sort_subset with s A1 A2 ; auto with coc core.
+  elim conv_sort_subset with s A1 A2 ; auto with coc core.
+
+  elim conv_prod_subset with B1 B2 A1 A2 ; auto with coc core.
+  elim conv_prod_subset with B1 B2 A1 A2 ; auto with coc core.
+
+  elim conv_sum_subset with B1 B2 A1 A2 ; auto with coc core.
+  elim conv_sum_subset with B1 B2 A1 A2 ; auto with coc core.
+
+  simpl in H0.
+  rewrite H2 ; unfold is_low_sort ; auto. 
+ 
+  simpl in H0.
+  apply (conv_is_low_range_full (inv_conv_subset_l _ _ _ _ H)).
+  rewrite H2 ; unfold is_low_sort ; auto.
+  rewrite H0 ; unfold is_low_sort ; auto.
+
+  induction B ; simpl ; intros ; 
+  try unfold is_low_sort in H1 ;   
+  intuition ; try discriminate ; auto with coc core datatypes.
+
+  elim conv_sort_subset with s A1 A2 ; auto with coc core.
+  elim conv_sort_subset with s A1 A2 ; auto with coc core.
+
+  elim conv_prod_subset with B1 B2 A1 A2 ; auto with coc core.
+  elim conv_prod_subset with B1 B2 A1 A2 ; auto with coc core.
+
+  elim conv_sum_subset with B1 B2 A1 A2 ; auto with coc core.
+  elim conv_sum_subset with B1 B2 A1 A2 ; auto with coc core.
+
+  simpl in H0.
+  apply (conv_is_low_range_full (inv_conv_subset_l _ _ _ _ H)).
+  rewrite H2 ; unfold is_low_sort ; auto.
+  rewrite H0 ; unfold is_low_sort ; auto.
+
+  simpl in H0.
+  rewrite H2 ; rewrite H0 ; auto.
 Qed.
-
+*)
 Lemma term_type_range_kinded : forall e t T, e |- t : T ->
   forall s, type_range t = Srt s -> T = Srt kind. 
 Proof.
@@ -1091,6 +635,19 @@ Proof.
   rewrite (IHtyp1 _ H3) in H1.
   elim typ_not_kind2 with e (Srt s) ; auto.
 Qed.
+(*
+Lemma term_type_dom_kinded : forall e t T, e |- t : T ->
+  forall s, type_dom t = Srt s -> T = Srt kind. 
+Proof.
+  induction 1 ; simpl ; intros ; try discriminate ; auto with coc.
+  
+  apply IHtyp2 with s ; auto.
+  apply IHtyp2 with s ; auto.
+  
+  rewrite (IHtyp1 _ H3) in H1.
+  elim typ_not_kind2 with e (Srt s) ; auto.
+Qed.
+*)
 
 Lemma type_range_sub : forall e T U s, e |- T >> U : s ->
   forall s0, type_range U = Srt s0 -> type_range T = Srt s0.
@@ -1128,11 +685,25 @@ Proof.
   pose (term_type_range_kinded t H1).
   discriminate.
 Qed.
+(*
+Lemma conv_ref_prod : forall n A B, ~ conv (Ref n) (Prod A B).
+Admitted.
+
+Lemma conv_ref_sum : forall n A B, ~ conv (Ref n) (Sum A B).
+Admitted.
+
+Lemma conv_abs_prod : forall T M A B, ~ conv (Abs T M) (Prod A B).
+Admitted.
+
+Lemma conv_abs_sum : forall T M A B, ~ conv (Abs T M) (Sum A B).
+Admitted.
+
 
 Lemma type_dom_sub : forall e T U s, e |- T >> U : s ->
   forall s0, type_dom U = Srt s0 -> type_dom T = Srt s0.
 Proof.
   induction 1 ; simpl ; intros ; try discriminate ; auto with coc.
+
   induction B ; try discriminate.
   simpl in H2.
   inversion H2.
@@ -1150,10 +721,40 @@ Proof.
   pose (term_type_range_kinded H3 H2).
   inversion e0.
   rewrite H6 in H3.
+
+  simpl.
+  rewrite H2.
   
+  pose (conv_is_low_dom_full).
+
+Focus 4.
+  pose (coerce_sym _ _ _ _ H).
+  exact (type_range_sub c H5).
+
+Focus 4.
+  exact (type_range_sub H H5).
+
+Focus 4.
+  pose (IHcoerce _ H1).
+  pose (coerce_sort_l _ _ _ _ H).
+  pose (term_type_range_kinded t e0).
   
-  apply (conv_is_low_range_full H1).
-  apply kind_is_prod with e (Srt s) ; auto.
+
+  induction A ; try discriminate.
+  
+  elim conv_sort_prod with s1 B1 B2 ; auto.
+  elim conv_ref_prod with n B1 B2 ; auto.
+  elim conv_abs_prod with A1 A2 B1 B2 ; auto.
+  simpl.
+  
+
+  apply IHB1.
+
+
+  apply (conv_is_low_dom_full H1).
+  
+
+apply kind_is_prod with e (Srt s) ; auto.
   apply kind_is_prod with e (Srt s) ; auto.
 
   rewrite <- H2.
@@ -1169,7 +770,31 @@ Proof.
   pose (term_type_range_kinded t H1).
   discriminate.
 Qed.
+Lemma var_sort_dom_item : forall e n T, e |- Ref n : T ->
+  forall s, type_dom T = (Srt s) -> 
+  exists T', item_lift T' e n /\ type_dom T' = Srt s.
+Admitted.
 
+Lemma unique_var_dom_sort : forall e n T, e |- Ref n : T ->
+  forall s, type_dom T = Srt s ->
+  forall T', e |- Ref n : T' -> 
+  forall s', type_dom T' = Srt s' -> s = s'.
+Proof.
+  intros.
+  destruct (var_sort_dom_item H H0).
+  destruct (var_sort_dom_item H1 H2).
+  destruct H3 ; destruct H4.
+  destruct H3 ; destruct H4.
+  pose (fun_item _ _ _ _ _ H7 H8).
+  rewrite <- e0 in H4.
+  rewrite <- H4 in H3.
+  rewrite <- H3 in H6.
+  rewrite H6 in H5.
+  inversion H5.
+  auto.
+Qed.
+
+*)
 
 Lemma var_sort_range_item_aux : forall e t T, e |- t : T ->
   forall n, t = Ref n -> 
@@ -1213,10 +838,6 @@ Proof.
   eapply var_sort_range_item_aux with (Ref n) T; auto ; auto.
 Qed.
 
-Lemma var_sort_dom_item : forall e n T, e |- Ref n : T ->
-  forall s, type_dom T = (Srt s) -> 
-  exists T', item_lift T' e n /\ type_dom T' = Srt s.
-Admitted.
 
 Lemma unique_var_sort : forall e n s, e |- Ref n : Srt s ->
   forall s', e |- Ref n : Srt s' -> s = s'.
@@ -1236,25 +857,6 @@ Proof.
   intros.
   destruct (var_sort_range_item H H0).
   destruct (var_sort_range_item H1 H2).
-  destruct H3 ; destruct H4.
-  destruct H3 ; destruct H4.
-  pose (fun_item _ _ _ _ _ H7 H8).
-  rewrite <- e0 in H4.
-  rewrite <- H4 in H3.
-  rewrite <- H3 in H6.
-  rewrite H6 in H5.
-  inversion H5.
-  auto.
-Qed.
-
-Lemma unique_var_dom_sort : forall e n T, e |- Ref n : T ->
-  forall s, type_dom T = Srt s ->
-  forall T', e |- Ref n : T' -> 
-  forall s', type_dom T' = Srt s' -> s = s'.
-Proof.
-  intros.
-  destruct (var_sort_dom_item H H0).
-  destruct (var_sort_dom_item H1 H2).
   destruct H3 ; destruct H4.
   destruct H3 ; destruct H4.
   pose (fun_item _ _ _ _ _ H7 H8).
@@ -1402,6 +1004,7 @@ Proof.
   apply sort_of_abs_range_aux with (Abs M N) Ts  ; auto ; auto.
 Qed.
 
+(*
 Lemma sort_of_abs_dom_aux : forall e t Ts, e |- t : Ts ->
   forall M N, t = Abs M N ->
   forall s, type_dom Ts = Srt s ->
@@ -1422,6 +1025,7 @@ Proof.
   apply (type_range_sub H2 H4).
 Qed.
 
+
 Lemma sort_of_abs_range : forall e M N Ts, e |- Abs M N : Ts ->
   forall s, type_range Ts = Srt s ->
   exists s1, exists s2, exists T, e |- M : (Srt s1) /\ M :: e |- N : T /\
@@ -1431,7 +1035,7 @@ Proof.
   apply sort_of_abs_range_aux with (Abs M N) Ts  ; auto ; auto.
 Qed.
 
-
+*)
 
 
 Lemma sort_of_pair_range_aux : forall e t Ts, e |- t : Ts ->
@@ -1447,11 +1051,11 @@ Proof.
   auto with coc core arith datatypes ; try discriminate.
 
   exists U ; exists V ; exists s1 ; exists s2.
-  inversion H3.
-  rewrite <- H7 ; rewrite <- H8.
+  inversion H4.
+  rewrite <- H9 ; rewrite <- H8.
   intuition.
   apply type_sum with s1 ; auto.
-  
+
   apply IHtyp1 ; auto.
   apply (type_range_sub H2 H4).
 Qed.
@@ -1468,26 +1072,129 @@ Proof.
   apply sort_of_pair_range_aux with (Pair T u v) Ts  ; auto ; auto.
 Qed.
 
+Lemma strength_sort_judgement : forall T e s s', T :: e |- Srt s : Srt s' ->
+  e |- Srt s : Srt s'.
+Proof.
+  intros.
+  pose (typ_wf _ _ _ H).
+  inversion w.
+  pose (typ_wf _ _ _ H1).
+  inversion H ; auto with coc.
+
+  destruct (typ_sort _ _ _ H).
+  inversion H11.
+  rewrite H13 in H4.
+  pose (type_has_no_kind H4).
+  simpl in t0.
+  intuition.
+Qed.
+
+Lemma type_sorted : forall e t T, e |- t : T ->
+  T = Srt kind \/ exists s, e |- T : Srt s.
+Proof.
+  induction 1 ; simpl ; intros ; auto with coc ; try discriminate ; 
+ try (destruct H ; discriminate) ;  try (destruct H1 ; discriminate).
+
+  right; exact (wf_sort_lift _ _ _ H H0).
+ 
+  right.
+  exists s2.
+  apply type_prod with s1 ; auto.
+
+  induction IHtyp2 ; try discriminate.
+  induction H1.
+  induction IHtyp1.
+  rewrite H2 in H0.
+  pose (type_no_kind_prod_type2 H0).
+  simpl in t.
+  intuition.
+
+  induction H2.
+  right.
+  exists x.
+  induction (generation_prod2 H1).
+  replace (Srt x) with (subst v (Srt x)).
+  apply (substitution _ _ _ _ H4 _ H).
+  unfold subst ; unfold subst_rec ; auto.
+
+  right.
+  exists s2.
+  apply type_sum with s1 ; auto.
+
+  induction IHtyp2.
+  left ; assumption.
+  induction H1.
+  right.
+  exists x ; auto.
+  eapply strength_sort_judgement with T ; auto.
+  
+  induction IHtyp2.
+  left ; auto.
+  induction H2.
+  right ; exists x ; auto.
+  eapply strength_sort_judgement with T ; auto.
+
+  induction IHtyp ; try discriminate.
+  induction H0.
+  induction (generation_sum2 H0).
+  destruct H1.
+  right ; exists x0 ; auto.
+
+  induction IHtyp ; try discriminate.
+  induction H0.
+  induction (generation_sum2 H0).
+  destruct H1.
+  destruct H2.
+  right.
+  exists x.
+  assert (e |- Pi1 t : U).
+  apply type_pi1 with V ; auto.
+  replace (Srt x) with (subst (Pi1 t) (Srt x)).
+  apply (substitution _ _ _ _ H2 _ H4).
+  unfold subst ; unfold subst_rec ; auto.
+  
+  right ; exists s ; auto.
+Qed.
+
 Lemma sort_of_pi1_range_aux : forall e t Ts, e |- t : Ts ->
   forall u, t = Pi1 u ->
   forall s, type_range Ts = Srt s ->
-  exists U, exists V, e |- u : Sum U V /\ type_range U = (Srt s).
+  exists U, exists V, exists s2, 
+  e |- u : Sum U V /\ type_range U = (Srt s)
+  /\ sum_sort U V s s2.
 Proof.
   induction 1 ; simpl ; intros ;
   auto with coc core arith datatypes ; try discriminate.
+  
+  induction (type_sorted H) ; try discriminate.
+  induction H2.
+  induction (generation_sum2 H2).
 
   exists U ; exists V.
   inversion H0.
-  rewrite <- H3.
+  rewrite <- H5.
+  exists x.
+  intuition.
+  pose (term_type_range_kinded H4 H1).
+  inversion e0.
+  rewrite H8 in H7.
+  unfold sum_sort in H7.
+  destruct H7.
+  induction H6 ; try discriminate.
+  unfold sum_sort.
   intuition.
   
+  destruct H6.
+  discriminate.
+
   apply IHtyp1 ; auto.
   apply (type_range_sub H2 H4).
 Qed.
 
 Lemma sort_of_pi1_range :  forall e t Ts, e |- Pi1 t : Ts ->
   forall s, type_range Ts = Srt s ->
-  exists U, exists V, e |- t : Sum U V /\ type_range U = (Srt s).
+  exists U, exists V, exists s2, e |- t : Sum U V /\ type_range U = (Srt s)
+  /\ sum_sort U V s s2.
 Proof.
   intros. 
   apply sort_of_pi1_range_aux with (Pi1 t) Ts  ; auto ; auto.
@@ -1527,12 +1234,12 @@ Lemma sort_of_letin_range_aux : forall e t Ts, e |- t : Ts ->
 Proof.
   induction 1 ; simpl ; intros ;
   auto with coc core arith datatypes ; try discriminate.
-
+  (*
   exists U ; exists M.
   inversion H3.
   rewrite <- H6 ; rewrite <- H7.
   intuition.
-  
+  *)
   apply IHtyp1 ; auto.
   apply (type_range_sub H2 H4).
 Qed.
@@ -1553,169 +1260,3 @@ Proof.
   induction t ; simpl ; intros ;
   auto with coc core arith datatypes ; try discriminate.
 Qed.
-
-Lemma unique_range_sort : forall t e T T', e |- t : T -> e |- t : T' -> 
-forall s1 s2, 
-(type_range T = Srt s1 -> type_range T' = Srt s2 -> s1 = s2) /\
-(type_dom T = Srt s1 -> type_dom T' = Srt s2 -> s1 = s2).
-Proof.
-  induction t ; simpl ; split ; intros ;
-  auto with coc core arith datatypes ; try discriminate.
-
-  destruct (typ_sort _ _ _ H).
-  destruct (typ_sort _ _ _ H0).
-  rewrite H4 in H1.
-  rewrite H6 in H2.
-  simpl in H1, H2.
-  inversion H2 ; inversion H1.
-  auto.
-
-  destruct (typ_sort _ _ _ H).
-  destruct (typ_sort _ _ _ H0).
-  rewrite H4 in H1.
-  rewrite H6 in H2.
-  simpl in H1, H2.
-  inversion H2 ; inversion H1.
-  auto.
-
-  (* Var *)
-  exact (unique_var_range_sort H H1 H0 H2).
-  exact (unique_var_dom_sort H H1 H0 H2).
-    
-  (* Abs *)
-  induction (sort_of_abs_range H H1).
-  do 2 destruct H3 ; intuition.
-  induction (sort_of_abs_range H0 H2).
-  do 2 destruct H6 ; intuition.
-
-  destruct (IHt2 _ _ _ H3 H6 s1 s2) ; simpl ; auto.
-
-
-  destruct (IHt2 _ _ _ H3 H6 s1 s2) ; simpl ; auto.
-
-
-  (* App goes well *)
-  induction (sort_of_app_range H H1).
-  destruct H3 ; intuition.
-  induction (sort_of_app_range H0 H2).
-  destruct H6 ; intuition.
-
-  apply (IHt1 _ _ _ H3 H6) ; simpl ; auto.
-
-  pose (term_type_range_kinded H4 H8).
-  rewrite e0 in H3.
-  pose (type_no_kind_prod_type2 H3).
-  simpl in t.
-  intuition.
-
-  induction (sort_of_app_range H0 H2).
-  destruct H6 ; intuition.
-
-  apply (IHt1 _ _ _ H3 H6) ; simpl ; auto.
-
-  pose (term_type_range_kinded H4 H5).
-  rewrite e0 in H3.
-  pose (type_no_kind_prod_type2 H3).
-  simpl in t.
-  intuition.
-
-  pose (term_type_range_kinded H4 H5).
-  rewrite e0 in H3.
-  pose (type_no_kind_prod_type2 H3).
-  simpl in t.
-  intuition.
-
-  (* Pair *)
-  induction (sort_of_pair_range H H1).
-  do 3 destruct H3 ; intuition.
-  induction (sort_of_pair_range H0 H2).
-  do 3 destruct H9 ; intuition.
-
-  apply (IHt3 _ _ _ H7 H14) ; simpl ; auto.
-  unfold subst ; apply type_range_subst2 ; auto.
-  unfold subst ; apply type_range_subst2 ; auto.
-  
-  (* Prod *)
-  induction (generation_prod H).
-  induction (generation_prod H0).
-  rewrite H3 in H.
-  rewrite H4 in H0.
-  induction (generation_prod2 H).
-  induction (generation_prod2 H0).
-  apply (IHt2 _ _ _ H6 H8).
-  rewrite <- H3 ; auto.
-  rewrite <- H4 ; auto.
-
-  (* Sum *)
-  induction (generation_sum H).
-  induction (generation_sum H0).
-  rewrite H3 in H.
-  rewrite H4 in H0.
-  induction (generation_sum2 H).
-  induction (generation_sum2 H0).
-  apply (IHt2 _ _ _ H6 H8).
-  rewrite <- H3 ; auto.
-  rewrite <- H4 ; auto.
-  
-  pose (generation_subset H).
-  pose (generation_subset H0).
-  rewrite e0 in H1.
-  rewrite e1 in H2.
-  simpl in H1 ; simpl in H2.
-  rewrite H2 in H1.
-  inversion H1 ; auto.
-
-  (* Pi1 *)
-  induction (sort_of_pi1_range H H1).
-  destruct H3 ; intuition.
-  induction (sort_of_pi1_range H0 H2).
-  destruct H3 ; intuition.
-
-  apply (IHt _ _ _ H4 H6) ; simpl ; auto.
-
-  pose (term_type_range_kinded H4 H8).
-  rewrite e0 in H3.
-  pose (type_no_kind_prod_type2 H3).
-  simpl in t.
-  intuition.
-
-  induction (sort_of_app_range H0 H2).
-  destruct H6 ; intuition.
-
-  apply (IHt1 _ _ _ H3 H6) ; simpl ; auto.
-
-  pose (term_type_range_kinded H4 H5).
-  rewrite e0 in H3.
-  pose (type_no_kind_prod_type2 H3).
-  simpl in t.
-  intuition.
-
-  pose (term_type_range_kinded H4 H5).
-  rewrite e0 in H3.
-  pose (type_no_kind_prod_type2 H3).
-  simpl in t.
-  intuition.
-
-
-
-Admitted. 
-(* Focus 3.
-
-  split.
-  intros.
-  apply trans_conv_conv with A ; auto with coc core.
-
-  intros.
-  apply trans_conv_conv with B ; auto with coc core.
-*)
-
-Theorem unique_sort : forall t e s s', 
-  e |- t : (Srt s) -> e |- t : (Srt s') -> s = s'.
-Proof.
-  intros.
-  exact (unique_range_sort H H0 (refl_equal (Srt s)) (refl_equal (Srt s'))).
-Qed.
-  
-  
-
-
